Move proof that well-formedness respects `sub_module` to sub_module.v
Fixup: Load ssreflect with fewer global side effects

theories/lang/cpp/logic/wp.v
@@ -712,67 +712,6 @@ Section with_cpp.
     : forall (tt : type_table) (fun_type : type) (ti : thread_info)
              (addr : val) (ls : list val) (Q : val -> epred), mpred.
 
-  Local Hint Constructors wf_decl wf_basic_type wf_type wf_pt_type wf_pt_types : core.
-
-  Lemma wf_decl_respects_GlobDecl_le {te g1 g2} :
-    GlobDecl_le g1 g2 = Some () ->
-    wf_decl te g1 ->
-    wf_decl te g2.
-  Proof.
-    intros Hle Hwf; inversion Hwf; simplify_eq; destruct g2 => //;
-      rewrite /= /require_eq in Hle;
-      case_decide => //; subst; auto.
-  Qed.
-
-  (* XXX Taken from sub_module. *)
-  Definition type_table_le (te1 te2 : type_table) : Prop :=
-    forall (gn : globname) gv,
-      te1 !! gn = Some gv ->
-      exists gv', te2 !! gn = Some gv' /\
-             GlobDecl_le gv gv' = Some tt.
-
-  Definition wf_decl_respects te2 g := ∀ te1,
-    type_table_le te2 te1 ->
-    wf_decl te1 g.
-  Definition wf_basic_type_respects te2 t := ∀ te1,
-    type_table_le te2 te1 ->
-    wf_basic_type te1 t.
-  Definition wf_pt_type_respects te2 t := ∀ te1,
-    type_table_le te2 te1 ->
-    wf_pt_type te1 t.
-  Definition wf_pt_types_respects te2 ts := ∀ te1,
-    type_table_le te2 te1 ->
-    wf_pt_types te1 ts.
-  Definition wf_type_respects te2 t := ∀ te1,
-    type_table_le te2 te1 ->
-    wf_type te1 t.
-
-  (* Actual mutual induction. *)
-  Lemma wf_respects_sub_table_mut te2 :
-    (∀ g : GlobDecl, wf_decl te2 g → wf_decl_respects te2 g) ∧
-    (∀ t : type, wf_basic_type te2 t → wf_basic_type_respects te2 t) ∧
-    (∀ t : type, wf_pt_type te2 t → wf_pt_type_respects te2 t) ∧
-    (∀ l : list type, wf_pt_types te2 l → wf_pt_types_respects te2 l) ∧
-    (∀ t : type, wf_type te2 t → wf_type_respects te2 t).
-  Proof.
-    apply wf_mut_ind; try solve [intros; red; repeat_on_hyps (fun H => red in H); eauto].
-    intros * Hlook Hwf IH ? Hsub.
-    destruct (Hsub _ _ Hlook) as (st1 & Hlook1 & Hle).
-    apply (wf_named_struct _ Hlook1).
-    apply (wf_decl_respects_GlobDecl_le Hle), IH, Hsub.
-  Qed.
-
-  Lemma wf_type_respects_sub_table te1 te2 t :
-    type_table_le te2 te1 ->
-    wf_type te2 t → wf_type te1 t.
-  Proof. intros. by eapply wf_respects_sub_table_mut. Qed.
-
-  Lemma wf_type_respects_sub_module tt1 tt2 t :
-    sub_module tt2 tt1 ->
-    wf_type tt2.(globals) t -> wf_type tt1.(globals) t.
-  Proof. move=> /types_compat Hsub Hwf. exact: wf_type_respects_sub_table. Qed.
-
-
   Axiom fspec_wf_type : forall te ft ti a ls Q,
       fspec te ft ti a ls Q
       |-- fspec te ft ti a ls Q **
